formalization/ett.v
@@ -136,7 +136,6 @@ with isterm : context -> term -> type -> Type :=
 
      | TermApp :
          forall {G A B u v},
-           istype (ctxextend G A) B ->
            isterm G u (Prod A B) ->
            isterm G v A ->
            isterm G (app u A B v) (Subst B (sbzero G A v))
